reverted to Finset, refactored types and proc constructors, extra types and dual properties, plus some renaminng

PiLL/PiLL/Definitions.lean
@@ -4,133 +4,144 @@ import Mathlib.Data.Finset.Card
 import Mathlib.Data.Finset.Fold
 ------------------------------------------ Proc  ------------------------------------------
 
-abbrev Name := String
-
-structure NonEmptyName where
-  (val : String)
-  (neEmpty : val ≠ "")                  -- val not empty
-  (no_spaces : ¬ (val.any (· = ' ')))   -- no spaces in val
-deriving Repr, BEq, DecidableEq
+abbrev PName := Nat -- Process names are just numbers (ensures not empty)
 
 inductive Proc : Type where
-  | tensor   : NonEmptyName → NonEmptyName → Proc → Proc -- x[y].P (output y on x and continue as P)
-  | parr     : NonEmptyName → NonEmptyName → Proc → Proc -- x(y).P (input y on x and continue as P)
-  | one      : NonEmptyName → Proc → Proc                -- x[].P
-  | bot      : NonEmptyName → Proc → Proc                -- x(y).P
-  | cut      : NonEmptyName → NonEmptyName → Proc → Proc -- 𝓋xy P (name restriction, or "cut")
-  | par      : Proc → Proc → Proc                        -- parallel composition of two processes
-  | nil      : Proc                                      -- terminated process
-deriving Repr
+  | tensor  (x y : PName) (P : Proc)   -- x[y].P
+  | parr    (x y : PName) (P : Proc)   -- x(y).P
+  | one     (x : PName) (P : Proc)     -- x[].P
+  | bot     (x : PName) (P : Proc)     -- x().P
+  | cut     (x y : PName) (P : Proc)   -- 𝒗xy P
+  | par     (P Q : Proc)               -- P | Q
+  | nil                                -- 𝟘
+deriving Repr, BEq, DecidableEq
 
 ------------------------------------------ TYPES  ------------------------------------------
 
-structure NonEmptyTypes where
-  val : String
-  restriction : Bool := val ≠ " " && val.all Char.isUpper || val = "∅"
-deriving Repr, BEq, DecidableEq
-
-def NonEmptyTypes.mkAuto (s : String) : NonEmptyTypes :=
-  { val := s }
-
-structure Atom where
-  (name : NonEmptyTypes)
-  (negated : Bool)
-deriving Repr, BEq, DecidableEq
-
-def Atom.mkAuto (s : String) (negated : Bool) : Atom :=
-  { name := NonEmptyTypes.mkAuto s, negated := negated }
-
-def Atom.neg (a : Atom) : Atom :=
-  { a with negated := !a.negated }
+abbrev Atom := Nat
 
 inductive Types : Type where
-  | term : Atom → Types                 -- named type, like A, B, ...
-  | tensor : Types → Types → Types      -- t₁ ⊗ t₂ (send)
-  | parr : Types → Types → Types        -- t₁ ⅋ t₂ (receive)
-  | one : Types                         -- 𝟙 (empty output, unit for ⊗)
-  | bot : Types                         -- ⊥ (empty send, unit for ⅋)
+  | atom      (a : Atom)      -- named type, like A, B, ...
+  | atomDual  (a : Atom)      -- dual of a named type
+  | tensor    (A B : Types)   -- t₁ ⊗ t₂ (send)
+  | parr      (A B : Types)   -- t₁ ⅋ t₂ (receive)
+  | one                       -- 𝟙 (empty output, unit for ⊗)
+  | bot                       -- ⊥ (empty send, unit for ⅋)
 deriving Repr, BEq, DecidableEq
 
-def neg : Types → Types
-| Types.tensor A B => Types.parr (neg A) (neg B)
-| Types.parr A B => Types.tensor (neg A) (neg B)
-| Types.one => Types.bot
-| Types.bot => Types.one
-| Types.term T => Types.term T.neg
+def Types.pos : Types → Prop
+  | atom _ => True
+  | one => True
+  | tensor _ _ => True
+  -- | oplus _ _ => True
+  -- | bang _ => True
+  -- | zero => True
+  | _ => False
+
+def Types.neg : Types → Prop
+  | atomDual _ => True
+  | bot => True
+  | parr _ _ => True
+  -- | top => True
+  -- | .with _ _ => True
+  -- | quest _ => True
+  | _ => False
+
+instance Types.posDecidable (A : Types) : Decidable A.pos := by
+  unfold Types.pos
+  split <;> infer_instance
+
+instance Types.negDecidable (A : Types) : Decidable A.neg := by
+  unfold Types.neg
+  split <;> infer_instance
+
+@[simp]
+def Types.dual : Types → Types
+| .tensor A B => .parr (dual A) (dual B)
+| .parr A B   => .tensor (dual A) (dual B)
+| .one        => .bot
+| .bot        => .one
+| .atom a     => .atomDual a
+| .atomDual a => .atom a
+
+@[simp]
+theorem Types.dual.neq (A : Types) : A ≠ dual A := by
+  cases A <;> simp [dual]
+
+@[simp]
+theorem dual.inj (A B : Types) : Types.dual A = Types.dual B ↔ A = B := by
+  induction A generalizing B <;> cases B <;> simp [Types.dual, *]
+
+@[simp]
+theorem dual.involution (A : Types) : Types.dual (Types.dual A) = A := by
+  induction A <;> simp [*]
 
 --------------------------------------- ENVIRONMENTS ---------------------------------------
 
-def upperCaseGreekLetters : List (Char) :=
-  ['Α', 'Β', 'Γ', 'Δ', 'Ε', 'Ζ', 'Η', 'Θ', 'Ι', 'Κ', 'Λ', 'Μ',
-  'Ν', 'Ξ', 'Ο', 'Π', 'Ρ', 'Σ', 'Τ', 'Υ', 'Φ', 'Χ', 'Ψ', 'Ω']
+abbrev Env := Finset (PName × Types)
 
-structure EnvNames where
-  (val : { s : String // s ≠ " " ∧ s.all (· ∈ upperCaseGreekLetters) })
-deriving Repr, BEq, DecidableEq
+abbrev EmptyEnv : Env := ∅
 
-abbrev Env := Finset (NonEmptyName × Types)
-
-abbrev EmptyEnv : Env := {}
-
-def Env.mk (x : NonEmptyName) (A : Types) : Env :=
+def Env.mk (x : PName) (A : Types) : Env :=
   {(x, A)}
 
-def envLinearity (Δ : Env) : Prop :=
+def Env.linear (Δ : Env) : Prop :=
   (Δ.image Prod.fst).card = Δ.card
 
-def getNamesInEnv (Δ : Env) : Finset (NonEmptyName) :=
+def Env.names (Δ : Env) : Finset (PName) :=
   (Δ.image Prod.fst)
 
-def disjointEnv (Δ Γ : Env) : Prop :=
+def Env.disjoint (Δ Γ : Env) : Prop :=
   (Δ.image Prod.fst ∩ Γ.image Prod.fst).card = 0
 
-noncomputable def envLookupTypeOf (Δ : Env) (x : NonEmptyName) : Option Types :=
+noncomputable def Env.lookup (Δ : Env) (x : PName) : Option Types :=
+  -- Finset.fold (· ∪ ·) none (fun p => if p.fst = x then p.snd else none) Δ
   (Δ.toList.find? (fun p => p.fst = x)).map Prod.snd
 
 -- Order independent equality for environments
-def envEq (Δ Γ : Env) : Prop :=
-  ∀ x : (NonEmptyName), envLookupTypeOf Δ x = envLookupTypeOf Γ x
+def Env.Eq (Δ Γ : Env) : Prop :=
+  ∀ x : (PName), Δ.lookup x = Γ.lookup x
 
 -- Eq reflexivity
 @[simp]
-theorem envEq.refl (Δ : Env) : envEq Δ Δ :=
+theorem Env.Eq_refl (Δ : Env) : Env.Eq Δ Δ :=
   fun _ => rfl
 
 -- Eq symmetry
 @[simp]
-theorem envEq.symm (Δ Γ : Env) (h : envEq Δ Γ) : envEq Γ Δ :=
+theorem Env.Eq_symm (Δ Γ : Env) (h : Env.Eq Δ Γ) : Env.Eq Γ Δ :=
   fun x => (h x).symm
 
 -- Eq transitivity
 @[simp]
-theorem envEq.trans (Δ Γ Ε : Env) (h₁ : envEq Δ Γ) (h₂ : envEq Γ Ε) : envEq Δ Ε :=
+theorem Env.Eq_trans (Δ Γ Ε : Env) (h₁ : Env.Eq Δ Γ) (h₂ : Env.Eq Γ Ε) : Env.Eq Δ Ε :=
   fun x => Eq.trans (h₁ x) (h₂ x)
 
-instance : Equivalence envEq :=
-⟨envEq.refl, @envEq.symm, @envEq.trans⟩
+instance : Equivalence Env.Eq :=
+⟨Env.Eq_refl, @Env.Eq_symm, @Env.Eq_trans⟩
 
-def mergeEnv (Δ Γ : Env) : Env := Δ ∪ Γ
+def Env.merge (Δ Γ : Env) : Env := Δ ∪ Γ
 
 -- identity
 @[simp]
-theorem mergeEnv.unitR (Δ : Env) : mergeEnv Δ EmptyEnv = Δ := by
-  simp [mergeEnv]
+theorem Env.merge_unitR (Δ : Env) : Δ.merge EmptyEnv = Δ := by
+  simp [Env.merge]
 
 @[simp]
-theorem mergeEnv.unitL (Δ : Env) : mergeEnv EmptyEnv Δ = Δ := by
-  simp [mergeEnv]
+theorem Env.merge_unitL (Δ : Env) : Env.merge EmptyEnv Δ = Δ := by
+  simp [Env.merge]
 
 -- commutivity
 -- theorem mergeEnv.comm (Δ Γ : Env) : disjointEnv Δ Γ → mergeEnv Δ Γ = mergeEnv Γ Δ := by
 @[simp]
-theorem mergeEnv.comm (Δ Γ : Env) : mergeEnv Δ Γ = mergeEnv Γ Δ := by
-  simp [mergeEnv]
+theorem Env.merge_comm (Δ Γ : Env) : Δ.merge Γ = Γ.merge Δ := by
+  simp [Env.merge]
   simp [Finset.union_comm]
 
 -- associativity
 @[simp]
-theorem mergeEnv.assoc (Δ Γ Ε : Env) : mergeEnv (mergeEnv Δ Γ) Ε = mergeEnv Δ (mergeEnv Γ Ε) := by
-  simp [mergeEnv]
+theorem Env.merge_assoc (Δ Γ Ε : Env) : (Δ.merge Γ).merge Ε = Δ.merge (Γ.merge Ε) := by
+  simp [Env.merge]
 
 ------------------------------------ HYPER-ENVIRONMENTS ------------------------------------
 
@@ -145,43 +156,43 @@ instance : Coe Env HyperEnv := ⟨fun Γ => {Γ}⟩
 def pairwise {α : Type} (r : α → α → Prop) (s : Finset α) : Prop :=
   ∀ x ∈ s, ∀ y ∈ s, y ≠ x → r x y
 
-def hyperEnvLinearity (𝒢 : HyperEnv) : Prop :=
-  ∀ Δ ∈ 𝒢, envLinearity Δ ∧                              -- ensure each env is linear
-  pairwise (fun Δ Γ => disjointEnv Δ Γ) 𝒢                -- ensure pairwise env disjointness
+def HyperEnv.linear (𝒢 : HyperEnv) : Prop :=
+  ∀ Δ ∈ 𝒢, Δ.linear ∧                               -- ensure each env is linear
+  pairwise (fun Δ Γ => Δ.disjoint Γ) 𝒢              -- ensure pairwise env disjointness
 
-def getNamesInHyperEnv (𝒢 : HyperEnv) : Finset NonEmptyName :=
-  Finset.fold (· ∪ ·) ∅ getNamesInEnv 𝒢
+def HyperEnv.names (𝒢 : HyperEnv) : Finset PName :=
+  Finset.fold (· ∪ ·) ∅ Env.names 𝒢
 
 -- Lookup method for finding the type of a name in the hyperenvironment
-noncomputable def hyperLookupTypeOf (𝒢 : HyperEnv) (x : NonEmptyName) : Option Types :=
-  (𝒢.toList.find? (fun Δ => envLookupTypeOf Δ x ≠ none)) >>= fun Δ  => envLookupTypeOf Δ x
+noncomputable def HyperEnv.lookup (𝒢 : HyperEnv) (x : PName) : Option Types :=
+  (𝒢.toList.find? (fun Δ => Δ.lookup x ≠ none)) >>= fun Δ  => Δ.lookup x
 
-def disjointHyperEnv (𝒢 ℋ : HyperEnv) : Prop :=
+def HyperEnv.disjoint (𝒢 ℋ : HyperEnv) : Prop :=
   -- 1. ensure both hyperenvs are lienar
   -- 2. ensure disjoint env names
   -- 3. ensure no duplicate definitions across hyperenvs
     -- s.t. an unambigous lookup in the individual hyperenvs
     -- yields an unambigous lookupin the merged hyperenv
     -- i.e. the intersection of their defined names is empty
-  hyperEnvLinearity 𝒢 ∧ hyperEnvLinearity ℋ ∧
+  𝒢.linear ∧ ℋ.linear ∧
   (𝒢 ∩ ℋ).card = 0 ∧
-  (getNamesInHyperEnv 𝒢 ∩ getNamesInHyperEnv ℋ) = ∅
+  (HyperEnv.names 𝒢 ∩ HyperEnv.names ℋ) = ∅
 
 -- Order independent equality for hyper-environments
-def hyperEnvEq (𝒢 ℋ : HyperEnv) : Prop :=
+def HyperEnv.Eq (𝒢 ℋ : HyperEnv) : Prop :=
   -- 𝒢 and ℋ must define the same names
-  getNamesInHyperEnv 𝒢 = getNamesInHyperEnv ℋ ∧
+  HyperEnv.names 𝒢 = HyperEnv.names ℋ ∧
   -- The typing of all defined names must match i.e. ∀ x, 𝒢(x) = ℋ(x)
-  ∀ x ∈ getNamesInHyperEnv 𝒢, hyperLookupTypeOf 𝒢 x = hyperLookupTypeOf ℋ x
+  ∀ x ∈ HyperEnv.names 𝒢, 𝒢.lookup x = ℋ.lookup x
 
 -- reflexivity
 @[simp]
-theorem hyperEnvEq.refl (𝒢 : HyperEnv) : hyperEnvEq 𝒢 𝒢 := by
-  simp [hyperEnvEq]
+theorem HyperEnv.Eq_refl (𝒢 : HyperEnv) : HyperEnv.Eq 𝒢 𝒢 := by
+  simp [HyperEnv.Eq]
 
 -- symmetry
 @[simp]
-theorem hyperEnvEq.symm (𝒢 ℋ : HyperEnv) (h : hyperEnvEq 𝒢 ℋ) : hyperEnvEq ℋ 𝒢 := by
+theorem HyperEnv.Eq_symm (𝒢 ℋ : HyperEnv) (h : HyperEnv.Eq 𝒢 ℋ) : HyperEnv.Eq ℋ 𝒢 := by
   rcases h with ⟨h_names, h_vals⟩
   refine ⟨h_names.symm, ?vals⟩
   intro x hx
@@ -190,42 +201,42 @@ theorem hyperEnvEq.symm (𝒢 ℋ : HyperEnv) (h : hyperEnvEq 𝒢 ℋ) : hyperE
 
 -- transitivity
 @[simp]
-theorem hyperEnvEq.trans (𝒢 ℋ 𝒦 : HyperEnv) (h₁ : hyperEnvEq 𝒢 ℋ) (h₂ : hyperEnvEq ℋ 𝒦) :
-  hyperEnvEq 𝒢 𝒦 := by
+theorem HyperEnv.Eq_trans (𝒢 ℋ 𝒦 : HyperEnv) (h₁ : HyperEnv.Eq 𝒢 ℋ) (h₂ : HyperEnv.Eq ℋ 𝒦) :
+  HyperEnv.Eq 𝒢 𝒦 := by
   rcases h₁ with ⟨h₁_names, h₁_vals⟩
   rcases h₂ with ⟨h₂_names, h₂_vals⟩
   refine ⟨?names, ?vals⟩
   · rw [h₁_names, h₂_names]
   · intro x hx
-    have hxH : x ∈ getNamesInHyperEnv ℋ := by rw [← h₁_names]; exact hx
+    have hxH : x ∈ ℋ.names := by rw [← h₁_names]; exact hx
     calc
-      hyperLookupTypeOf 𝒢 x = hyperLookupTypeOf ℋ x := h₁_vals x hx
-      _    = hyperLookupTypeOf 𝒦 x := h₂_vals x hxH
+      𝒢.lookup x = ℋ.lookup x := h₁_vals x hx
+      _    = 𝒦.lookup x := h₂_vals x hxH
 
-instance : Equivalence hyperEnvEq :=
-⟨hyperEnvEq.refl, @hyperEnvEq.symm, @hyperEnvEq.trans⟩
+instance : Equivalence HyperEnv.Eq :=
+⟨HyperEnv.Eq_refl, @HyperEnv.Eq_symm, @HyperEnv.Eq_trans⟩
 
-noncomputable def mergeHyperEnv (𝒢 ℋ : HyperEnv) : HyperEnv := 𝒢 ∪ ℋ
+noncomputable def HyperEnv.merge (𝒢 ℋ : HyperEnv) : HyperEnv := 𝒢 ∪ ℋ
 
 -- identity
 @[simp]
-theorem mergeHyperEnv.unitL (𝒢 : HyperEnv) : mergeHyperEnv EmptyHyperEnv 𝒢 = 𝒢 := by
-  simp [mergeHyperEnv]
+theorem mergeHyperEnv.unitL (𝒢 : HyperEnv) : HyperEnv.merge EmptyHyperEnv 𝒢 = 𝒢 := by
+  simp [HyperEnv.merge]
 
 @[simp]
-theorem mergeHyperEnv.unitR (𝒢 : HyperEnv) : mergeHyperEnv 𝒢 EmptyHyperEnv = 𝒢 := by
-  simp [mergeHyperEnv]
+theorem mergeHyperEnv.unitR (𝒢 : HyperEnv) : HyperEnv.merge 𝒢 EmptyHyperEnv = 𝒢 := by
+  simp [HyperEnv.merge]
 
 -- commutative
 @[simp]
-theorem mergeHyperEnv.comm (𝒢 ℋ : HyperEnv) : mergeHyperEnv 𝒢 ℋ = mergeHyperEnv ℋ 𝒢 := by
-  simp [mergeHyperEnv, Finset.union_comm]
+theorem mergeHyperEnv.comm (𝒢 ℋ : HyperEnv) : HyperEnv.merge 𝒢 ℋ = HyperEnv.merge ℋ 𝒢 := by
+  simp [HyperEnv.merge, Finset.union_comm]
 
 -- associativity
 @[simp]
 theorem mergeHyperEnv.assoc (𝒢 ℋ 𝒦 : HyperEnv) :
-  mergeHyperEnv (mergeHyperEnv 𝒢 ℋ) 𝒦 = mergeHyperEnv 𝒢 (mergeHyperEnv ℋ 𝒦) := by
-  simp [mergeHyperEnv]
+  HyperEnv.merge (HyperEnv.merge 𝒢 ℋ) 𝒦 = HyperEnv.merge 𝒢 (HyperEnv.merge ℋ 𝒦) := by
+  simp [HyperEnv.merge]
 
 ----------------------------------------- NOTATION -----------------------------------------
 
@@ -243,15 +254,15 @@ infixr:95 " ⊗ " => Types.tensor
 infixr:95 " ⅋ " => Types.parr
 notation:100 "𝟙" => Types.one
 notation:100 "⊥" => Types.bot
-notation:max A "ᗮ" => neg A
+notation:max A "ᗮ" => Types.dual A
 
 /- ENV -/
 infixr:90 " ∶ " => Env.mk
-infixr:85 "‚ " => mergeEnv
+infixr:85 "‚ " => Env.merge
 
 /- HYPERENV -/
-notation:60 𝒢 "⸨" x "⸩" => hyperLookupTypeOf 𝒢 x
-infixr:55 " |ₕ " => mergeHyperEnv
+notation:60 𝒢 "⸨" x "⸩" => HyperEnv.lookup 𝒢 x
+infixr:55 " |ₕ " => HyperEnv.merge
 
 --------------------------------------- TYPING RULES ---------------------------------------
 
@@ -265,73 +276,70 @@ inductive Typing : HyperEnv → Proc → Prop where
     --------------------------
      Typing (𝒢 |ₕ ℋ) (P |ₚ Q)
 
-  | cut (𝒢 : HyperEnv) (Γ Δ : Env) (P : Proc) (x y : NonEmptyName) (A : Types) :
+  | cut (𝒢 : HyperEnv) (Γ Δ : Env) (P : Proc) (x y : PName) (A : Types) :
     Typing (𝒢 |ₕ Γ‚ x ∶ A |ₕ Δ‚ y ∶ Aᗮ) P →
     ---------------------------------------
         Typing (𝒢 |ₕ Γ‚ Δ) (𝑣⸨x, y⸩ P)
 
-  | tensor (Γ Δ : Env) (P : Proc) (x y : NonEmptyName) (A B : Types) :
+  | tensor (Γ Δ : Env) (P : Proc) (x y : PName) (A B : Types) :
     Typing (Γ‚ y ∶ A |ₕ Δ‚ x ∶ B) P →
     ---------------------------------
     Typing (Γ‚ Δ‚ x ∶ A ⊗ B) (x⟦y⟧.P)
 
-  | one (P : Proc) (x : NonEmptyName) :
+  | one (P : Proc) (x : PName) :
         Typing ∅ P →
     --------------------
     Typing (x ∶ 𝟙) (x⟦⟧.P)
 
-  | parr (Γ : Env) (P : Proc) (x y : NonEmptyName) (A B : Types) :
+  | parr (Γ : Env) (P : Proc) (x y : PName) (A B : Types) :
      Typing (Γ‚ y ∶ A‚ x ∶ B) P →
     -----------------------------
     Typing (Γ‚ x ∶ A ⅋ B) (x⸨y⸩.P)
 
-  | bot (Γ : Env) (P : Proc) (x : NonEmptyName) :
+  | bot (Γ : Env) (P : Proc) (x : PName) :
           Typing Γ P →
     ------------------------
     Typing (Γ‚ x ∶ ⊥) (x⸨⸩.P)
 
 notation:50 "⊢ " P " ∷ " T => Typing T P
 
-variable (x y z : NonEmptyName)
-set_option pp.notation false in -- disable pretty print
-#check Proc.cut x y (Proc.par (Proc.one x 𝟘) (Proc.bot y (Proc.one z 𝟘)))
-set_option pp.notation false in -- disable pretty print
-#check 𝑣⸨x , y⸩ x⟦⟧.𝟘 |ₚ y⸨⸩.z⟦⟧.𝟘
 
-example (x y z : NonEmptyName) : ⊢ 𝑣⸨x , y⸩ x⟦⟧.𝟘 |ₚ y⸨⸩.z⟦⟧.𝟘 ∷ ∅ |ₕ ∅ |ₕ z ∶ 𝟙 := by
-  apply Typing.cut ∅ ∅ (z ∶ 𝟙) _ _ _ (𝟙)
-  rw [mergeHyperEnv.unitL]
-  apply Typing.mix
-  · apply Typing.one
-    exact Typing.mix₀
-  · apply Typing.bot
-    apply Typing.one
-    exact Typing.mix₀
+
+
+-- inductive πLL : Type where
+--   | sorry
+
+
+
+
+
+
+
+
+
+---------------------------------------- EXAMPLES ----------------------------------------
 
 -- Latch_xyz example from main.pdf
 -- TODO: Try and use simp more, try and omit giving explicit types to cut,
 --       in general try minimizing things given to cut
-example (x x₁ x₂ y y₁ y₂ z : NonEmptyName) :
+example (x x₁ x₂ y y₁ y₂ z : PName) :
   ⊢ 𝑣⸨x₁, x₂⸩ 𝑣⸨y₁, y₂⸩ x⸨⸩.x₁⟦⟧.𝟘 |ₚ y⸨⸩.y₁⟦⟧.𝟘 |ₚ x₂⸨⸩.y₂⸨⸩.z⟦⟧.𝟘 ∷
     x ∶ ⊥‚ y ∶ ⊥‚ z ∶ 𝟙 := by
   apply Typing.cut ∅ _ _ _ _ _ (𝟙)
-  rw [mergeHyperEnv.unitL, mergeEnv.comm]
-  conv => lhs ; rhs ; rhs ; rw [mergeEnv.assoc]
+  rw [mergeHyperEnv.unitL, Env.merge_comm]
+  conv => lhs ; rhs ; rhs ; rw [Env.merge_assoc]
   apply Typing.cut _ _ _ _ _ _ (𝟙)
   apply Typing.mix
   · apply Typing.bot
     apply Typing.one
     exact Typing.mix₀
   · apply Typing.mix
-    · rw [mergeEnv.comm]
+    · rw [Env.merge_comm]
       apply Typing.bot
       apply Typing.one
       exact Typing.mix₀
-    · conv => lhs ; rhs ; rw [mergeEnv.comm, ←mergeEnv.assoc] ; lhs ; rw [mergeEnv.comm]
+    · conv => lhs ; rhs ; rw [Env.merge_comm, ←Env.merge_assoc] ; lhs ; rw [Env.merge_comm]
       apply Typing.bot
       apply Typing.bot
       apply Typing.one
       exact Typing.mix₀
-
--- inductive πLL : Type where
---   | sorry
