PiLL/PiLL/3AListAttempt.lean
@@ -1,0 +1,393 @@
+----------------------------------------- imports -----------------------------------------
+import Mathlib.Data.Finset.Basic
+import Mathlib.Data.Finset.Card
+import Mathlib.Data.Finset.Fold
+import Mathlib.Data.List.AList
+------------------------------------------ Proc  ------------------------------------------
+
+abbrev PName := Nat -- Process names are just numbers (ensures not empty)
+
+inductive Proc : Type where
+  | tensor  (x y : PName) (P : Proc)   -- x[y].P
+  | parr    (x y : PName) (P : Proc)   -- x(y).P
+  | one     (x : PName) (P : Proc)     -- x[].P
+  | bot     (x : PName) (P : Proc)     -- x().P
+  | cut     (x y : PName) (P : Proc)   -- 𝒗xy P
+  | par     (P Q : Proc)               -- P | Q
+  | nil                                -- 𝟘
+deriving Repr, BEq, DecidableEq
+
+------------------------------------------ TYPES  ------------------------------------------
+universe u
+
+variable {Atom : Type u}
+
+inductive Types (Atom : Type u) : Type u where
+  | atom    (a : Atom)            -- A, B, ... (A typing term)
+  | atomDual (a : Atom)           -- The dual of A, B ...
+  | tensor  (A B : Types Atom)    -- t₁ ⊗ t₂ (send)
+  | parr    (A B : Types Atom)    -- t₁ ⅋ t₂ (receive)
+  | one                           -- 𝟙 (empty output, unit for ⊗)
+  | bot                           -- ⊥ (empty send, unit for ⅋)
+deriving Repr, BEq, DecidableEq
+
+instance : Bot (Types Atom) := ⟨.bot⟩
+instance : One (Types Atom) := ⟨.one⟩
+
+-- TODO: define which Types are positive / negative
+-- TODO: decidability for positive / negative propositions
+
+def Types.pos : Types Atom → Prop
+  | atom _ => True
+  | one => True
+  | tensor _ _ => True
+  -- | oplus _ _ => True
+  -- | bang _ => True
+  -- | zero => True
+  | _ => False
+
+def Types.neg : Types Atom → Prop
+  | atomDual _ => True
+  | bot => True
+  | parr _ _ => True
+  -- | top => True
+  -- | .with _ _ => True
+  -- | quest _ => True
+  | _ => False
+
+instance Types.posDecidable (A : Types Atom) : Decidable A.pos := by
+  unfold Types.pos
+  split <;> infer_instance
+
+instance Types.negDecidable (A : Types Atom) : Decidable A.neg := by
+  unfold Types.neg
+  split <;> infer_instance
+
+@[simp]
+def Types.dual : Types Atom → Types Atom
+| .tensor A B => .parr (dual A) (dual B)
+| .parr A B   => .tensor (dual A) (dual B)
+| .one        => .bot
+| .bot        => .one
+| .atom a     => .atomDual a
+| .atomDual a => .atom a
+
+@[simp]
+theorem Types.dual.neq (A : Types Atom) : A ≠ dual A := by
+  cases A <;> simp [dual]
+
+@[simp]
+theorem dual.inj (A B : Types Atom) : Types.dual A = Types.dual B ↔ B = A := by
+  induction A generalizing B <;> cases B
+  all_goals aesop
+
+@[simp]
+theorem dual.involution (A : Types Atom) : Types.dual (Types.dual A) = A := by
+  induction A <;> simp [*]
+
+--------------------------------------- ENVIRONMENTS ---------------------------------------
+
+abbrev Env Atom := AList (fun (_ : PName) => Types Atom)
+
+instance envDecidableEq {Atom : Type} [DecidableEq Atom] : DecidableEq (Env Atom) :=
+  AList.instDecidableEq
+
+abbrev EmptyEnv : Env Atom := (∅ : AList (fun (_ : PName) => Types Atom))
+
+def Env.mk (x : PName) (A : Types Atom) : Env Atom :=
+  (List.toAList []).insert x A
+
+def Env.names (Δ : Env Atom) : List (PName) :=
+  Δ.keys
+
+-- Order independent equality for environments
+@[simp]
+def envEq (Δ Γ : Env Atom) : Prop :=
+  ∀ (x : PName), Δ.lookup x = Γ.lookup x
+
+-- Eq reflexivity
+@[simp]
+theorem envEq.refl (Δ : Env Atom) : envEq Δ Δ :=
+  fun _ => rfl
+
+-- Eq symmetry
+@[simp]
+theorem envEq.symm (Δ Γ : Env Atom) (h : envEq Δ Γ) : envEq  Γ Δ :=
+  fun x => (h x).symm
+
+-- Eq transitivity
+@[simp]
+theorem envEq.trans (Δ Γ Ε : Env Atom) (h₁ : envEq Δ Γ) (h₂ : envEq Γ Ε) :
+  envEq  Δ Ε := fun x => Eq.trans (h₁ x) (h₂ x)
+
+instance {Atom : Type} : Equivalence (@envEq Atom) :=
+{ refl := @envEq.refl Atom,
+  symm := @envEq.symm Atom,
+  trans := @envEq.trans Atom }
+
+-- Missing sorting to make cannonical form
+-- Missing disjoint requirement
+@[simp]
+-- def Env.merge (Δ Γ : Env Atom) [Decidable (Δ.Disjoint Γ)] : Option (Env Atom) :=
+--   if Δ.Disjoint Γ then some (Δ ∪ Γ) else none
+def Env.merge {Atom : Type u} (Δ Γ : Env Atom) (h : AList.Disjoint Δ Γ) : Env Atom :=
+  Δ ∪ Γ
+
+-- identity
+@[simp]
+theorem mergeEnv.unitR {Atom : Type u} (Δ : Env Atom) :
+    Δ.merge EmptyEnv (by intro k ; simp [AList.keys_empty]) = Δ := by
+  simp
+
+@[simp]
+theorem mergeEnv.unitL {Atom : Type u} (Δ : Env Atom) :
+    EmptyEnv.merge Δ (by intro k ; simp [AList.keys_empty]) = Δ := by
+  trivial
+
+-- commutivity
+@[simp]
+theorem mergeEnv.comm (Δ Γ : Env Atom) (h : AList.Disjoint Δ Γ) :
+  (Δ.merge Γ h).entries.Perm (Γ.merge Δ (by intro k hk h' ; exact h k h' hk)).entries :=
+  AList.union_comm_of_disjoint h
+
+-- associativity
+@[simp]
+theorem mergeEnv.assoc {Atom : Type u}
+  (Δ Γ Ε : Env Atom)
+  (hΔΓ : Δ.Disjoint Γ)
+  (hΔΓΕ : Δ.Disjoint (Γ ∪ Ε))
+  (hΓΕ : Γ.Disjoint Ε)
+  (hΕΔΓ : Ε.Disjoint (Δ ∪ Γ)) :
+  (Ε.merge (Δ.merge Γ hΔΓ) hΕΔΓ).entries.Perm
+  (Δ.merge (Γ.merge Ε hΓΕ) hΔΓΕ).entries := by
+  unfold Env.merge
+  -- exact AList.union_assoc
+  sorry -- The above should work but there is some DecidableEq thing Lean gets stuck on
+
+------------------------------------ HYPER-ENVIRONMENTS ------------------------------------
+
+abbrev HyperEnv Atom := Finset (Env Atom)
+
+abbrev EmptyHyperEnv : HyperEnv Atom := {}
+
+-- Coercion makes extending a hyperenv with env and merging the same
+-- and env1 |ₕ env2 => hyperenv due to envs being lifted to hyperenv
+instance : Coe (Env Atom) (HyperEnv Atom) := ⟨fun Γ => {Γ}⟩
+
+-- def pairwise {α : Type} (r : α → α → Prop) (s : Finset α) : Prop :=
+--   ∀ x ∈ s, ∀ y ∈ s, y ≠ x → r x y
+
+def hyperEnv.linearity (𝒢 : HyperEnv Atom) : Prop :=
+  -- ∀ Δ ∈ 𝒢, envLinearity Δ ∧                              -- ensure each env is linear
+  -- pairwise (fun Δ Γ => AList.Disjoint Δ Γ) 𝒢              -- ensure pairwise env disjointness
+  ∀ x ∈ 𝒢, ∀ y ∈ 𝒢, y ≠ x → x.Disjoint y
+
+def HyperEnv.names (𝒢 : HyperEnv Atom) : Finset PName :=
+  Finset.fold (· ∪ ·) ∅ (fun Δ => Δ.names.toFinset) 𝒢
+
+-- Lookup method for finding the type of a name in the hyperenvironment
+noncomputable def hyperLookupTypeOf (𝒢 : HyperEnv Atom) (x : PName) : Option (Types Atom) :=
+  (𝒢.toList.find? (fun Δ => (Δ.lookup x).isSome)) >>= fun Δ  => Δ.lookup x
+
+def HyperEnv.disjoint (𝒢 ℋ : HyperEnv Atom) [DecidableEq (Env Atom)] : Prop :=
+  -- 1. ensure both hyperenvs are lienar
+  -- 2. ensure disjoint env names
+  -- 3. ensure no duplicate definitions across hyperenvs
+    -- s.t. an unambigous lookup in the individual hyperenvs
+    -- yields an unambigous lookupin the merged hyperenv
+    -- i.e. the intersection of their defined names is empty
+  hyperEnv.linearity 𝒢 ∧ hyperEnv.linearity ℋ ∧
+  (𝒢 ∩ ℋ).card = 0 ∧
+  (HyperEnv.names 𝒢 ∩ HyperEnv.names ℋ) = ∅
+
+-- Order independent equality for hyper-environments
+def hyperEnv.Eq (𝒢 ℋ : HyperEnv Atom) : Prop :=
+  -- 𝒢 and ℋ must define the same names
+  HyperEnv.names 𝒢 = HyperEnv.names ℋ ∧
+  -- The typing of all defined names must match i.e. ∀ x, 𝒢(x) = ℋ(x)
+  ∀ x ∈ HyperEnv.names 𝒢, hyperLookupTypeOf 𝒢 x = hyperLookupTypeOf ℋ x
+
+-- reflexivity
+@[simp]
+theorem hyperEnvEq.refl (𝒢 : HyperEnv Atom) : hyperEnv.Eq 𝒢 𝒢 := by
+  simp [hyperEnv.Eq]
+
+-- symmetry
+@[simp]
+theorem hyperEnvEq.symm (𝒢 ℋ : HyperEnv Atom) (h : hyperEnv.Eq 𝒢 ℋ) : hyperEnv.Eq ℋ 𝒢 := by
+  rcases h with ⟨h_names, h_vals⟩
+  refine ⟨h_names.symm, ?vals⟩
+  intro x hx
+  rw [h_names] at h_vals
+  apply (h_vals x hx).symm
+
+-- transitivity
+@[simp]
+theorem hyperEnvEq.trans (𝒢 ℋ 𝒦 : HyperEnv Atom) (h₁ : hyperEnv.Eq 𝒢 ℋ) (h₂ : hyperEnv.Eq ℋ 𝒦) :
+  hyperEnv.Eq 𝒢 𝒦 := by
+  rcases h₁ with ⟨h₁_names, h₁_vals⟩
+  rcases h₂ with ⟨h₂_names, h₂_vals⟩
+  refine ⟨?names, ?vals⟩
+  · rw [h₁_names, h₂_names]
+  · intro x hx
+    have hxH : x ∈ HyperEnv.names ℋ := by rw [← h₁_names]; exact hx
+    calc
+      hyperLookupTypeOf 𝒢 x = hyperLookupTypeOf ℋ x := h₁_vals x hx
+      _    = hyperLookupTypeOf 𝒦 x := h₂_vals x hxH
+
+instance {Atom : Type} : Equivalence (@hyperEnv.Eq Atom) :=
+{ refl := @hyperEnvEq.refl Atom,
+  symm := @hyperEnvEq.symm Atom,
+  trans := @hyperEnvEq.trans Atom }
+
+@[simp]
+noncomputable def HyperEnv.merge (𝒢 ℋ : HyperEnv Atom) [DecidableEq (Env Atom)] : HyperEnv Atom :=
+  𝒢 ∪ ℋ
+
+-- identity
+@[simp]
+theorem mergeHyperEnv.unitL (𝒢 : HyperEnv Atom) [DecidableEq (Env Atom)] :
+  HyperEnv.merge EmptyHyperEnv 𝒢 = 𝒢 := by
+  simp
+
+@[simp]
+theorem mergeHyperEnv.unitR (𝒢 : HyperEnv Atom) [DecidableEq (Env Atom)] :
+  HyperEnv.merge 𝒢 EmptyHyperEnv = 𝒢 := by
+  simp
+
+-- commutative
+@[simp]
+theorem mergeHyperEnv.comm (𝒢 ℋ : HyperEnv Atom) [DecidableEq (Env Atom)] :
+  HyperEnv.merge 𝒢 ℋ = HyperEnv.merge ℋ 𝒢 := by
+  simp [Finset.union_comm]
+
+-- associativity
+@[simp]
+theorem mergeHyperEnv.assoc (𝒢 ℋ 𝒦 : HyperEnv Atom) [DecidableEq (Env Atom)] :
+  HyperEnv.merge (HyperEnv.merge 𝒢 ℋ) 𝒦 = HyperEnv.merge 𝒢 (HyperEnv.merge ℋ 𝒦) := by
+  simp
+----------------------------------------- NOTATION -----------------------------------------
+
+/- PROC -/
+notation:80 x "⟦" y "⟧" "." P:80 => Proc.tensor x y P
+notation:80 x "⟦" "⟧" "." P:80 => Proc.one x P
+notation:80 x "⸨" y "⸩" "." P:80 => Proc.parr x y P
+notation:80 x "⸨" "⸩" "." P:80 => Proc.bot x P
+notation:60 "𝑣" "⸨" x ", " y "⸩ " P => Proc.cut x y P
+notation "𝟘" => Proc.nil
+infixr:65 " |ₚ " => Proc.par
+
+/- TYPING -/
+
+-- -- TAKE A LOOK AT THIS COMPARED TO WHAT YOU HAVE:
+-- @[inherit_doc] scoped infix:35 " ⊗ " => Proposition.tensor
+-- @[inherit_doc] scoped infix:35 " ⊕ " => Proposition.oplus
+-- @[inherit_doc] scoped infix:30 " ⅋ " => Proposition.parr
+-- @[inherit_doc] scoped infix:30 " & " => Proposition.with
+
+-- @[inherit_doc] scoped prefix:95 "!" => Proposition.bang
+-- @[inherit_doc] scoped prefix:95 "ʔ" => Proposition.quest
+
+infixr:95 " ⊗ " => Types.tensor
+infixr:95 " ⅋ " => Types.parr
+notation:100 "𝟙" => Types.one
+notation:100 "⊥" => Types.bot
+notation:max A "ᗮ" => Types.dual A
+
+/- ENV -/
+infixr:90 " ∶ " => Env.mk
+infixr:85 "‚ " => Env.merge
+
+/- HYPERENV -/
+notation:60 𝒢 "⸨" x "⸩" => hyperLookupTypeOf 𝒢 x
+infixr:55 " |ₕ " => HyperEnv.merge
+
+--------------------------------------- TYPING RULES ---------------------------------------
+
+-- inductive Typing : HyperEnv Atom → Proc → Prop where
+--   | mix₀ :
+--     ----------
+--     Typing ∅ 𝟘
+
+--   | mix (𝒢 ℋ : HyperEnv Atom) (P Q : Proc) :
+--     Typing 𝒢 P → Typing ℋ Q →
+--     --------------------------
+--      Typing (𝒢 |ₕ ℋ) (P |ₚ Q)
+
+--   | cut (𝒢 : HyperEnv Atom) (Γ Δ : Env Atom) (P : Proc) (x y : PName) (A : Types Atom) :
+--     Typing (𝒢 |ₕ Γ‚ x ∶ A |ₕ Δ‚ y ∶ Aᗮ) P →
+--     ---------------------------------------
+--         Typing (𝒢 |ₕ Γ‚ Δ) (𝑣⸨x, y⸩ P)
+
+--   | tensor (Γ Δ : Env Atom) (P : Proc) (x y : PName) (A B : Types Atom) :
+--     Typing (Γ‚ y ∶ A |ₕ Δ‚ x ∶ B) P →
+--     ---------------------------------
+--     Typing (Γ‚ Δ‚ x ∶ A ⊗ B) (x⟦y⟧.P)
+
+--   | one (P : Proc) (x : PName) :
+--         Typing ∅ P →
+--     --------------------
+--     Typing (x ∶ 𝟙) (x⟦⟧.P)
+
+--   | parr (Γ : Env Atom) (P : Proc) (x y : PName) (A B : Types Atom) :
+--      Typing (Γ‚ y ∶ A‚ x ∶ B) P →
+--     -----------------------------
+--     Typing (Γ‚ x ∶ A ⅋ B) (x⸨y⸩.P)
+
+--   | bot (Γ : Env Atom) (P : Proc) (x : PName) :
+--           Typing Γ P →
+--     ------------------------
+--     Typing (Γ‚ x ∶ ⊥) (x⸨⸩.P)
+
+-- notation:50 "⊢ " P " ∷ " T => Typing T P
+
+-- variable (x y z : PName)
+-- set_option pp.notation false in -- disable pretty print
+-- #check Proc.cut x y (Proc.par (Proc.one x 𝟘) (Proc.bot y (Proc.one z 𝟘)))
+
+
+
+-- -- inductive LTS : Type where
+-- --   | sorry
+
+
+
+
+
+
+
+
+
+
+
+
+
+
+
+
+-- ----------------------------------------- EXAMPLES -----------------------------------------
+
+-- -- Latch_xyz example from main.pdf
+-- -- TODO: Try and use simp more, try and omit giving explicit types to cut,
+-- --       in general try minimizing things given to cut
+-- example (x x₁ x₂ y y₁ y₂ z : PName) :
+--   ⊢ 𝑣⸨x₁, x₂⸩ 𝑣⸨y₁, y₂⸩ x⸨⸩.x₁⟦⟧.𝟘 |ₚ y⸨⸩.y₁⟦⟧.𝟘 |ₚ x₂⸨⸩.y₂⸨⸩.z⟦⟧.𝟘 ∷
+--     x ∶ ⊥‚ y ∶ ⊥‚ z ∶ 𝟙 := by
+--   apply Typing.cut ∅ _ _ _ _ _ (𝟙)
+--   rw [mergeHyperEnv.unitL, mergeEnv.comm]
+--   conv => lhs ; rhs ; rhs ; rw [mergeEnv.assoc]
+--   apply Typing.cut _ _ _ _ _ _ (𝟙)
+--   apply Typing.mix
+--   · apply Typing.bot
+--     apply Typing.one
+--     exact Typing.mix₀
+--   · apply Typing.mix
+--     · rw [mergeEnv.comm]
+--       apply Typing.bot
+--       apply Typing.one
+--       exact Typing.mix₀
+--     · conv => lhs ; rhs ; rw [mergeEnv.comm, ←mergeEnv.assoc] ; lhs ; rw [mergeEnv.comm]
+--       apply Typing.bot
+--       apply Typing.bot
+--       apply Typing.one
+--       exact Typing.mix₀
